nat proof stuff

Veir/Dialects/ModArith/ModArith.lean
@@ -5,35 +5,38 @@ namespace Veir.Dialects.ModArith
 /--
   Barrett reduction requires that the input value is less than `m^2` and that `m > 0`.
 -/
-def BarretPrecondition (m x : Nat) : Prop :=
-  0 < m ∧ x < m * m
+def BarretPrecondition (m x k : Nat) : Prop :=
+  0 < m ∧ x < m * m ∧ 2 ^ k > m
 
 /--
   Barrett-reducing a value in [0, m^2) should yield a value in [0, 2m)
    that is either `x mod m` or `x mod m + m`.
 -/
-def BarrettReduceSpec (m x r : Nat) : Prop :=
-    BarretPrecondition m x →
+def BarrettReduceSpec (m x k r : Nat) : Prop :=
+    BarretPrecondition m x k →
     (r = x % m ∨ r = x % m + m)
 
 /--
   If a value is Barrett-reduced,
   the result is less than twice the modulus.
 -/
-theorem BarretReduceSpecImpliesLt2q (m x r : Nat) :
-  (BarretPrecondition m x ∧
-  BarrettReduceSpec m x r ) →
+theorem BarretReduceSpecImpliesLt2q (m x k r : Nat) :
+  (BarretPrecondition m x k ∧
+  BarrettReduceSpec m x k r ) →
     r < 2 * m := by
     rintro ⟨hBounds, hSpec⟩
     have hOr := hSpec hBounds
     have hlt := Nat.mod_lt x hBounds.left
-    grind
+    omega
 
-theorem barrettReduceStepNatCorrect (m x : Nat) :
-  ∀ output, barrettReduceStepNat m x = output  →
-    BarrettReduceSpec m x output := by
-    intro output hOutput
-    simp [BarrettReduceSpec, BarretPrecondition]
-    intro h0 hmm
-    unfold barrettReduceStepNat at hOutput
+theorem barrettReduceStepNatCorrect (m x k : Nat) :
+  ∀ output, barrettReduceStepNat m x k = output  →
+    BarrettReduceSpec m x k output := by
+    -- intro output hOutput
+    -- simp [BarrettReduceSpec, BarretPrecondition]
+    -- intro h0 hmm
+    -- unfold barrettReduceStepNat at hOutput
+    unfold barrettReduceStepNat BarrettReduceSpec BarretPrecondition
+    simp
+    -- grind [Nat.mod_def, Nat.div_eq_sub_mod_div]
     sorry
